src/tls/Handshake.fsti
@@ -92,7 +92,7 @@ type session = {
 val prepareClientHello: config -> KeySchedule.ks -> option ri -> option sessionID -> ST ch
   (requires (fun h -> True))
   (ensures (fun h0 i h1 -> True))
-val prepareServerHello: config -> KeySchedule.ks -> option ri -> ch -> ST (result (sh * nego))
+val prepareServerHello: config -> KeySchedule.ks -> option ri -> ch -> ST (result (sh * nego * option CommonDH.key))
   (requires (fun h -> True))
   (ensures (fun h0 i h1 -> True))
 val processServerHello: c:config -> KeySchedule.ks -> option ri -> ch -> sh ->
